\noindent \textred{3.} Solve the recurrence:
$$ T(n) = 2T(\sqrt{n}) + (\log  \log  n)^2 $$
(Hint: How to make change of variables so that you can apply Masterâ€™s method?)
\newline \\
\textblue{
If we set $m = \log  n$, so $n = 2^m$, we have
$$ T(2^m) = 2 T(\sqrt{2^m}) + \log  m = 2 T(2^{\frac{m}{2}}) + (\log  m)^2 $$
Then we let $S(m) = T(2^m)$, we have
$$ S(m) = 2 S(\frac{m}{2}) + (\log  m)^2 $$
which is in the form of
$$ S(m) = a S(\frac{m}{b}) + f(m), $$
where $a = 2$, $b = 2$ and $f(m) = (\log m)^2$. Since we know that
$$ \log m = O(\sqrt{m}), $$
we can also show that 
$$ f(m) = (\log m)^2 = O(m) = m^{\log _b a}$$
Therefore, we can readily apply Master's method and get the solution:
$$ S(m) = \Theta(m) \implies \underline{T(n) = \Theta(\log n)} $$
}